# RDF Schema file for the MIDI map LV2 extension
#
# This document describes the classes and properties that are defined by the
# MIDI map extension to the LV2 specification.

@prefix ll:   <http://ll-plugins.nongnu.org/lv2/namespace#> .
@prefix lv2:  <http://lv2plug.in/ontology#> .
@prefix rdf:  <http://www.w3.org/1999/02/22-rdf-syntax-ns#> .
@prefix rdfs: <http://www.w3.org/2000/01/rdf-schema#> .


# The host feature instance for this extension
ll:midimap-ext
  a lv2:HostFeature;
  rdfs:comment """
This extension allows the plugin writer to specify MIDI controllers that
the host should map to control input ports. For example, a synth plugin that
has a control input port with index 5 that controls the gain of the synth 
could map this input port to MIDI CC 7 ("Channel Volume"). The host would 
then filter out all CC events with controller number 7 that comes in to the
default MIDI port (specified using the ll:defaultMidiPort property defined 
below) and for each such event, set the value of control input port 5 to the
value of the controller event (mapped to the range of the control port).

If no default MIDI port is specified, the host should assume that the
control rate input port with datatype ll:miditype with the lowest index is
the default MIDI port. If there are no such ports, the plugin does not have
a default MIDI port. The host may (optionally) still use the MIDI controller
mappings, for example by creating a "virtual" MIDI port for the plugin 
instance that does not correspond to an actual plugin port, but is only used 
to receive controller events that can be mapped to control input ports.

The mappings defined by this extensions should be viewed as default values. The
host may change these mappings for a plugin instance at any time.

This extension consists only of the specified RDF classes and properties, there
is no code or data structures. When passing the LV2_Host_Feature struct for
this extension to the instantiate() function for a plugin the 'data' member
should be set to NULL.
""".


####################################################################
# Classes                                                          #
####################################################################

ll:MidiController
  a rdfs:Class;
  rdfs:label "MIDI Controller";
  rdfs:comment """
This class represents a MIDI controller, either a CC number or a NRPN
number. In order for it to be considered valid by a host it must have
exactly one occurance of each of the following properties:
  ll:controllerType (with object ll:CC or ll:NRPN)
  ll:controllerNumber (with an integer literal as object, in the range 
                       0-127 for ll:CC or 0-16383 for ll:NRPN)
""".

ll:MidiControllerType
  a rdfs:Class;
  rdfs:label "MIDI Controller Type";
  rdfs:comment """
This class represents a MIDI controller type. The only two valid instances
of this class are ll:CC and ll:NRPN.
""".


####################################################################
# Properties                                                       #
####################################################################

ll:defaultMidiPort
  a rdf:Property;
  rdfs:domain  lv2:Plugin;
  rdfs:label   "Default MIDI port";
  rdfs:comment """
Used to define the default MIDI port for a plugin. The object should be an
integer literal that is the port index for the port that should be the 
default MIDI port. This port must be a control rate input port with the 
datatype <http://ll-plugins.nongnu.org/lv2/namespace#miditype>.
""".

ll:defaultMidiController
  a rdf:Property;
  rdfs:domain  lv2:Port;
  rdfs:range   ll:MidiController;
  rdfs:label   "Default MIDI controller";
  rdfs:comment """
Associates control input port with MIDI controllers. The subject port must 
be a control rate input port with the datatype lv2:float.
""".

ll:controllerType
  a rdf:Property;
  rdfs:domain  ll:MidiController;
  rdfs:range   ll:MidiControllerType;
  rdfs:label   "MIDI controller type";
  rdfs:comment "The type of this controller. Either ll:CC or ll:NRPN.".

ll:controllerNumber
  a rdf:Property;
  rdfs:domain  ll:MidiController;
  rdfs:label   "MIDI controller number";
  rdfs:comment """
The number for this controller. Should be in the range 0-127 for ll:CC or
0-16383 for ll:NRPN.
""".


####################################################################
# Instances                                                        #
####################################################################

ll:CC 
  a ll:controllerType;
  rdfs:label "MIDI CC";
  rdfs:comment "MIDI CC controller type".

ll:NRPN 
  a ll:controllerType;
  rdfs:label "MIDI NRPN";
  rdfs:comment "MIDI NRPN controller type".

